Add an example to the demo

tests/src/demo.rs
@@ -112,3 +112,14 @@ impl Counter for usize {
 pub fn use_counter<'a, T: Counter>(cnt: &'a mut T) -> usize {
     cnt.incr()
 }
+
+/* Cryptographic example */
+fn mod_add(a: u32, b: u32) -> u32 {
+    assert!( a < 3329 );
+    assert!( b < 3329 );
+    let sum = a + b;
+    let res = sum.wrapping_sub(3329);
+    let mask = res >> 16;
+    let q = 3329 & mask;
+    res.wrapping_add(q)
+}
